Finish refactoring brute force proof

theories/MaxOfTwoNumbers/Theorems/Attempt_01_BruteForce.v
@@ -1,41 +1,27 @@
 From Coq Require Import Floats Sint63 Uint63 QArith Lia List PArray Derive.
 From NeuralNetInterp.Torch Require Import Tensor Einsum Slicing.
-From NeuralNetInterp Require Import max_parameters max max_heuristics.
 From NeuralNetInterp.Util Require Import Pointed.
 From NeuralNetInterp.Util.Arith Require Import Classes Instances FloatArith.
 From NeuralNetInterp.Torch Require Import Tensor.Instances.
-From NeuralNetInterp Require Import max_instances.
-From NeuralNetInterp Require Import max_all_logits.
+From NeuralNetInterp.MaxOfTwoNumbers Require Import Parameters Model Heuristics TheoremStatement Model.Instances.
+From NeuralNetInterp.MaxOfTwoNumbers.Computed Require Import AllLogits.
 Local Open Scope uint63_scope.
 Local Open Scope core_scope.
-
-Definition total : int := Eval vm_compute in Shape.item (Shape.reshape (shape_of all_tokens)).
-Definition expected_correct : int := Eval vm_compute in total - Uint63.of_Z (List.length heuristics.incorrect_results).
-Definition totalf : float := Eval vm_compute in PrimFloat.of_uint63 total.
-Definition expected_correctf : float := Eval vm_compute in PrimFloat.of_uint63 expected_correct.
-Definition expected_accuracy : float := Eval vm_compute in expected_correctf / totalf.
-
-Definition real_accuracy : float
-  := Tensor.item (acc_fn (return_per_token := false) (logits all_tokens) all_tokens).
-
-Set NativeCompute Timing.
 
 Derive computed_accuracy SuchThat (computed_accuracy = real_accuracy) As computed_accuracy_eq.
 Proof.
   cbv [real_accuracy].
   etransitivity; revgoals.
   { apply Tensor.item_Proper; intro.
-    eapply acc_fn_Proper; repeat intro; subst.
-    2-3: reflexivity.
+    eapply Model.acc_fn_Proper; repeat intro; subst; [ | reflexivity .. ].
     apply all_tokens_logits_eq. }
   Time vm_compute; reflexivity.
 Defined.
 
-Definition error : float := Eval cbv in (20 / totalf)%float.
 Compute abs (computed_accuracy - expected_accuracy). (*      = 0.0023193359375%float *)
 Compute (abs (computed_accuracy - expected_accuracy) * totalf)%float. (* = 19 *) (* probably from floating point assoc issues, etc *)
 Compute Qred (PrimFloat.to_Q (computed_accuracy * totalf)) / Qred (PrimFloat.to_Q totalf). (*      = 8154 # 8192 *)
-Theorem good_accuracy : (abs (real_accuracy - expected_accuracy) <? error)%float = true.
+Theorem good_accuracy : TheoremStatement.Accuracy.best (* (abs (real_accuracy - expected_accuracy) <? error)%float = true *).
 Proof.
   rewrite <- computed_accuracy_eq.
   vm_compute; reflexivity.
