theories/MaxOfTwoNumbers/Model/Instances.v
@@ -1,0 +1,44 @@
+From Coq Require Import Morphisms RelationClasses.
+From NeuralNetInterp.Util Require Import Default (* Pointed PArray PArray.Instances Wf_Uint63.Instances List Notations Arith.Classes Arith.Instances Bool*) SolveProperEqRel.
+(*From NeuralNetInterp.Util.Tactics Require Import DestructHead.*)
+(*From NeuralNetInterp.Util Require Nat Wf_Uint63.*)
+From NeuralNetInterp.Torch Require Import Tensor Tensor.Instances Slicing Slicing.Instances.
+From NeuralNetInterp.TransformerLens Require Import HookedTransformer HookedTransformer.Instances.
+From NeuralNetInterp.MaxOfTwoNumbers Require Import Model.
+(*
+Import Util.Nat.Notations.
+Import Util.Wf_Uint63.LoopNotation.
+Import Util.Wf_Uint63.
+Import Util.Wf_Uint63.Reduction.
+Import Arith.Instances.Truncating.
+Local Open Scope float_scope.
+Local Open Scope list_scope.
+*)
+(*Import ListNotations.
+Local Open Scope raw_tensor_scope.
+#[local] Generalizable All Variables.*)
+
+Module Model.
+  Export Model.
+
+  #[export] Instance embed_Proper {r batch pos} : Proper (Tensor.eqf ==> Tensor.eqf) (@embed r batch pos)
+    := _.
+  #[export] Instance pos_embed_Proper {r batch pos} : Proper (Tensor.eqf ==> Tensor.eqf) (@pos_embed r batch pos)
+    := _.
+  #[export] Instance ln_final_Proper {r batch pos} : Proper (Tensor.eqf ==> Tensor.eqf) (@ln_final r batch pos)
+    := _.
+  #[export] Instance unembed_Proper {r batch pos} : Proper (Tensor.eqf ==> Tensor.eqf) (@unembed r batch pos)
+    := _.
+  #[export] Instance logits_Proper {r batch pos} : Proper (Tensor.eqf ==> Tensor.eqf) (@logits r batch pos)
+    := _.
+  Notation model_Proper := logits_Proper (only parsing).
+
+  #[export] Instance loss_fn_Proper {r batch return_per_token}
+    : Proper (Tensor.eqf ==> Tensor.eqf ==> Tensor.eqf) (@loss_fn r batch return_per_token).
+  Proof. cbv [loss_fn]; HookedTransformer.t. Qed.
+
+  #[export] Instance acc_fn_Proper {r batch return_per_token}
+    : Proper (Tensor.eqf ==> Tensor.eqf ==> Tensor.eqf) (@acc_fn r batch return_per_token).
+  Proof. cbv [acc_fn]; HookedTransformer.t. Qed.
+End Model.
+Export (hints) Model.
