theories/TransformerLens/HookedTransformer/Instances.v
@@ -1,0 +1,291 @@
+From Coq Require Import Floats Sint63 Uint63 QArith Lia List PArray Morphisms RelationClasses.
+From NeuralNetInterp.Util Require Import Default Pointed PArray PArray.Instances Wf_Uint63.Instances List Notations Arith.Classes Arith.Instances Bool SolveProperEqRel.
+From NeuralNetInterp.Util.Tactics Require Import DestructHead.
+From NeuralNetInterp.Util Require Nat Wf_Uint63.
+From NeuralNetInterp.Torch Require Import Tensor Tensor.Instances Einsum Slicing Slicing.Instances.
+From NeuralNetInterp.TransformerLens Require Import HookedTransformer.
+Import Util.Nat.Notations.
+Import Util.Wf_Uint63.LoopNotation.
+Import Util.Wf_Uint63.
+Import Util.Wf_Uint63.Reduction.
+Import Arith.Instances.Truncating.
+Local Open Scope float_scope.
+Local Open Scope list_scope.
+Set Implicit Arguments.
+Import ListNotations.
+Local Open Scope raw_tensor_scope.
+#[local] Generalizable All Variables.
+
+Module HookedTransformer.
+  Export HookedTransformer.
+
+  Ltac t_step :=
+    first [ match goal with
+            | [ |- ?x = ?x ] => reflexivity
+            | [ |- PArray.checkpoint _ _ = PArray.checkpoint _ _ ]
+              => apply Tensor.PArray.checkpoint_Proper
+            | [ |- Tensor.of_bool _ _ = Tensor.of_bool _ _ ]
+              => apply Tensor.of_bool_Proper
+            | [ |- Tensor.map2 _ _ _ _ = Tensor.map2 _ _ _ _ ]
+              => apply Tensor.map2_Proper
+           | [ |- Tensor.map2' _ _ _ _ = Tensor.map2' _ _ _ _ ]
+             => apply (Tensor.map2'_Proper (RA:=eq) (RB:=eq))
+            | [ |- Tensor.map _ _ _ = Tensor.map _ _ _ ]
+              => apply Tensor.map_Proper
+            | [ |- Tensor.map' _ _ _ = Tensor.map' _ _ _ ]
+              => apply (Tensor.map'_Proper (RA:=eq))
+            | [ |- Tensor.squeeze _ _ = Tensor.squeeze _ _ ]
+              => apply Tensor.squeeze_Proper
+            | [ |- reduce_axis_m1 _ _ _ = reduce_axis_m1 _ _ _ ]
+              => apply @Tensor.reduce_axis_m1_Proper with (RA:=eq)
+            | [ |- Tensor.gather_dim_m1 _ _ _ = Tensor.gather_dim_m1 _ _ _ ]
+              => apply Tensor.gather_dim_m1_Proper
+            | [ |- Tensor.softmax_dim_m1 _ _ = Tensor.softmax_dim_m1 _ _ ]
+              => apply Tensor.softmax_dim_m1_Proper
+            | [ |- Tensor.log_softmax_dim_m1 _ _ = Tensor.log_softmax_dim_m1 _ _ ]
+              => apply Tensor.log_softmax_dim_m1_Proper
+            | [ |- Tensor.mean _ _ = Tensor.mean _ _ ]
+              => apply Tensor.mean_Proper
+            | [ |- Tensor.where_ _ _ _ _ = Tensor.where_ _ _ _ _ ]
+              => apply Tensor.where__Proper
+            | [ |- Tensor.repeat _ _ _ = Tensor.repeat _ _ _ ]
+              => apply Tensor.repeat_Proper
+            | [ |- ?R (@SliceIndex.slice ?A ?ri ?ro ?idxs ?s _ _) (@SliceIndex.slice ?A ?ri ?ro ?idxs ?s _ _) ]
+              => eapply (@SliceIndex.slice_Proper A ri ro idxs s R)
+            | [ |- ?R (@FancyIndex.slice ?A ?rb ?sb ?ri ?ro ?idxs ?s _ _) (@FancyIndex.slice ?A ?rb ?sb ?ri ?ro ?idxs' ?s _ _) ]
+              => eapply (@FancyIndex.slice_Proper A rb sb ri ro)
+            | [ |- Reduction.argmax _ _ _ _ = Reduction.argmax _ _ _ _ ]
+              => apply Reduction.argmax_Proper_pointwise
+            | [ |- Reduction.mean _ _ _ _ = Reduction.mean _ _ _ _ ]
+              => apply Reduction.mean_Proper_pointwise
+            | [ |- Reduction.max _ _ _ _ = Reduction.max _ _ _ _ ]
+              => apply Reduction.max_Proper_pointwise
+            | [ |- Reduction.sum _ _ _ _ = Reduction.sum _ _ _ _ ]
+              => apply Reduction.sum_Proper_pointwise
+            | [ |- Reduction.prod _ _ _ _ = Reduction.prod _ _ _ _ ]
+              => apply Reduction.prod_Proper_pointwise
+            | [ |- FancyIndex.t_relation _ _ ] => constructor
+            | [ |- FancyIndexType_relation _ _ ] => hnf
+            | [ |- ((_ + _) ?idx = (_ + _) ?idx)%core ]
+              => apply (Tensor.tensor_add_Proper (RA:=eq) (RB:=eq))
+            | [ |- ((_ - _) ?idx = (_ - _) ?idx)%core ]
+              => apply (Tensor.tensor_sub_Proper (RA:=eq) (RB:=eq))
+            | [ |- ((_ * _) ?idx = (_ * _) ?idx)%core ]
+              => apply (Tensor.tensor_mul_Proper (RA:=eq) (RB:=eq))
+            | [ |- ((_ / _) ?idx = (_ / _) ?idx)%core ]
+              => apply (Tensor.tensor_div_by_Proper (RA:=eq) (RB:=eq))
+            | [ |- ((sqrt _) ?idx = (sqrt _) ?idx)%core ]
+              => apply Tensor.tensor_sqrt_Proper
+            | [ |- ((- _) ?idx = (- _) ?idx)%core ]
+              => apply Tensor.tensor_opp_Proper
+            | [ |- (_ + _ = _ + _)%core ] => apply f_equal2
+            | [ |- (_ * _ = _ * _)%core ] => apply f_equal2
+            | [ |- (_ - _ = _ - _)%core ] => apply f_equal2
+            | [ |- (_ / _ = _ / _)%core ] => apply f_equal2
+            | [ H : Tensor.eqfR ?R ?x ?y |- ?R (?x ?i) (?y ?i) ]
+              => apply H
+            | [ H : pointwise_relation _ ?R ?f ?g |- ?R (?f _) (?g _) ]
+              => apply H
+            | [ H : respectful _ ?R ?f ?g |- ?R (?f _) (?g _) ]
+              => apply H
+            end
+          | intro
+          | progress cbv [sqr]
+          | match goal with
+            | [ |- context[match ?x with _ => _ end] ] => destruct x
+            end ].
+
+  Ltac t := repeat t_step.
+
+  Module Embed.
+    Export Embed.
+
+    #[export] Instance forward_Proper {A d_vocab d_model W_E r s}
+      : Proper (Tensor.eqf ==> Tensor.eqf) (@forward A d_vocab d_model W_E r s).
+    Proof. cbv [forward]; t. Qed.
+  End Embed.
+  Export (hints) Embed.
+
+  Module Unembed.
+    Export Unembed.
+
+    #[export] Instance forward_Proper {A addA mulA zeroA d_model d_vocab_out W_U b_U r batch_pos}
+      : Proper (Tensor.eqf ==> Tensor.eqf) (@forward A addA mulA zeroA d_model d_vocab_out W_U b_U r batch_pos).
+    Proof. cbv [forward]; t. Qed.
+  End Unembed.
+  Export (hints) Unembed.
+
+  Module PosEmbed.
+    Export PosEmbed.
+
+    #[export] Instance forward_Proper {A d_model n_ctx W_pos r batch tokens_length}
+      : Proper (Tensor.eqf ==> Tensor.eqf) (@forward A d_model n_ctx W_pos r batch tokens_length).
+    Proof. cbv [forward]; t. Qed.
+  End PosEmbed.
+  Export (hints) PosEmbed.
+
+  Module LayerNorm.
+    Export LayerNorm.
+
+    #[export] Instance linpart_Proper {r A s d_model addA subA divA zeroA coerZ}
+      : Proper (Tensor.eqf ==> Tensor.eqf) (@linpart r A s d_model addA subA divA zeroA coerZ).
+    Proof. cbv [linpart]; t. Qed.
+
+    #[export] Instance scale_Proper {r A s d_model addA mulA divA sqrtA zeroA coerZ eps}
+      : Proper (Tensor.eqf ==> Tensor.eqf) (@scale r A s d_model addA mulA divA sqrtA zeroA coerZ eps).
+    Proof. cbv [scale]; t. Qed.
+
+    #[export] Instance rescale_Proper {r A s d_model divA}
+      : Proper (Tensor.eqf ==> Tensor.eqf ==> Tensor.eqf) (@rescale r A s d_model divA).
+    Proof. cbv [rescale]; t. Qed.
+
+    #[export] Instance postrescale_Proper {r A s d_model addA mulA w b}
+      : Proper (Tensor.eqf ==> Tensor.eqf) (@postrescale r A s d_model addA mulA w b).
+    Proof. cbv [postrescale]; t. Qed.
+
+    #[export] Instance forward_Proper {r A s d_model addA subA mulA divA sqrtA zeroA coerZ default eps w b}
+      : Proper (Tensor.eqf ==> Tensor.eqf) (@forward r A s d_model addA subA mulA divA sqrtA zeroA coerZ default eps w b).
+    Proof.
+      cbv [forward]; repeat first [ t_step | apply postrescale_Proper | apply rescale_Proper | apply scale_Proper | apply linpart_Proper ].
+    Qed.
+  End LayerNorm.
+  Export (hints) LayerNorm.
+
+  Module Attention.
+    Export Attention.
+
+    #[export] Instance einsum_input_Proper {A r batch addA zeroA mulA pos n_heads d_model d_head use_split_qkv_input}
+      : Proper (Tensor.eqf ==> Tensor.eqf ==> Tensor.eqf) (@einsum_input A r batch addA zeroA mulA pos n_heads d_model d_head use_split_qkv_input).
+    Proof. cbv [einsum_input]; t. Qed.
+
+    #[export] Instance q_Proper {A r batch addA zeroA mulA defaultA pos n_heads d_model d_head use_split_qkv_input W_Q b_Q}
+      : Proper (Tensor.eqf ==> Tensor.eqf) (@q A r batch addA zeroA mulA defaultA pos n_heads d_model d_head use_split_qkv_input W_Q b_Q).
+    Proof. cbv [q]; repeat first [ t_step | apply einsum_input_Proper ]. Qed.
+
+    #[export] Instance k_Proper {A r batch addA zeroA mulA defaultA pos n_heads d_model d_head use_split_qkv_input W_Q b_Q}
+      : Proper (Tensor.eqf ==> Tensor.eqf) (@k A r batch addA zeroA mulA defaultA pos n_heads d_model d_head use_split_qkv_input W_Q b_Q).
+    Proof. cbv [k]; repeat first [ t_step | apply einsum_input_Proper ]. Qed.
+
+    #[export] Instance v_Proper {A r batch addA zeroA mulA defaultA pos n_heads d_model d_head use_split_qkv_input W_Q b_Q}
+      : Proper (Tensor.eqf ==> Tensor.eqf) (@v A r batch addA zeroA mulA defaultA pos n_heads d_model d_head use_split_qkv_input W_Q b_Q).
+    Proof. cbv [v]; repeat first [ t_step | apply einsum_input_Proper ]. Qed.
+
+    #[export] Instance attn_scores_Proper {A r batch sqrtA coerZ addA zeroA mulA divA defaultA pos n_heads d_model d_head use_split_qkv_input W_Q W_K b_Q b_K}
+      : Proper (Tensor.eqf ==> Tensor.eqf ==> Tensor.eqf) (@attn_scores A r batch sqrtA coerZ addA zeroA mulA divA defaultA pos n_heads d_model d_head use_split_qkv_input W_Q W_K b_Q b_K).
+    Proof. cbv [attn_scores]; repeat first [ t_step | apply q_Proper | apply k_Proper ]. Qed.
+
+    #[export] Instance apply_causal_mask_Proper {A r batch coerZ pos n_heads n_ctx}
+      : Proper (Tensor.eqf ==> Tensor.eqf) (@apply_causal_mask A r batch coerZ pos n_heads n_ctx).
+    Proof. cbv [apply_causal_mask]; t. Qed.
+
+    #[export] Instance masked_attn_scores_Proper {A r batch sqrtA coerZ addA zeroA mulA divA defaultA pos n_heads d_model d_head n_ctx use_split_qkv_input W_Q W_K b_Q b_K}
+      : Proper (Tensor.eqf ==> Tensor.eqf ==> Tensor.eqf) (@masked_attn_scores A r batch sqrtA coerZ addA zeroA mulA divA defaultA pos n_heads d_model d_head n_ctx use_split_qkv_input W_Q W_K b_Q b_K).
+    Proof. cbv [masked_attn_scores]; repeat first [ t_step | apply apply_causal_mask_Proper | apply attn_scores_Proper ]. Qed.
+
+    #[export] Instance pattern_Proper {A r batch sqrtA coerZ addA zeroA mulA divA expA defaultA pos n_heads d_model d_head n_ctx use_split_qkv_input W_Q W_K b_Q b_K}
+      : Proper (Tensor.eqf ==> Tensor.eqf ==> Tensor.eqf) (@pattern A r batch sqrtA coerZ addA zeroA mulA divA expA defaultA pos n_heads d_model d_head n_ctx use_split_qkv_input W_Q W_K b_Q b_K).
+    Proof. cbv [pattern]; repeat first [ t_step | apply masked_attn_scores_Proper ]. Qed.
+
+    #[export] Instance z_Proper {A r batch sqrtA coerZ addA zeroA mulA divA expA defaultA pos n_heads d_model d_head n_ctx use_split_qkv_input W_Q W_K W_V b_Q b_K b_V}
+      : Proper (Tensor.eqf ==> Tensor.eqf ==> Tensor.eqf ==> Tensor.eqf) (@z A r batch sqrtA coerZ addA zeroA mulA divA expA defaultA pos n_heads d_model d_head n_ctx use_split_qkv_input W_Q W_K W_V b_Q b_K b_V).
+    Proof.
+      cbv [z]; t.
+      { apply v_Proper; t. }
+      { apply pattern_Proper; t. }
+    Qed.
+
+    #[export] Instance attn_out_Proper {A r batch sqrtA coerZ addA zeroA mulA divA expA defaultA pos n_heads d_model d_head n_ctx use_split_qkv_input W_Q W_K W_V W_O b_Q b_K b_V b_O}
+      : Proper (Tensor.eqf ==> Tensor.eqf ==> Tensor.eqf ==> Tensor.eqf) (@attn_out A r batch sqrtA coerZ addA zeroA mulA divA expA defaultA pos n_heads d_model d_head n_ctx use_split_qkv_input W_Q W_K W_V W_O b_Q b_K b_V b_O).
+    Proof. cbv [attn_out]; repeat first [ t_step | apply z_Proper ]. Qed.
+  End Attention.
+  Export (hints) Attention.
+
+  Module TransformerBlock.
+    Export TransformerBlock.
+
+    #[export] Instance add_head_dimension_Proper {A r batch pos n_heads d_model use_split_qkv_input}
+      : Proper (Tensor.eqf ==> Tensor.eqf) (@add_head_dimension A r batch pos n_heads d_model use_split_qkv_input).
+    Proof. cbv [add_head_dimension]; t. Qed.
+
+    #[export] Instance query_input_Proper {A r batch pos n_heads d_model use_split_qkv_input}
+      : Proper (Tensor.eqf ==> Tensor.eqf) (@query_input A r batch pos n_heads d_model use_split_qkv_input)
+      := _.
+    #[export] Instance key_input_Proper {A r batch pos n_heads d_model use_split_qkv_input}
+      : Proper (Tensor.eqf ==> Tensor.eqf) (@key_input A r batch pos n_heads d_model use_split_qkv_input)
+      := _.
+    #[export] Instance value_input_Proper {A r batch pos n_heads d_model use_split_qkv_input}
+      : Proper (Tensor.eqf ==> Tensor.eqf) (@value_input A r batch pos n_heads d_model use_split_qkv_input)
+      := _.
+
+    #[export] Instance ln1_Proper {A zeroA coerZ addA subA mulA divA sqrtA default d_model eps ln1_w ln1_b r s}
+      : Proper (Tensor.eqf ==> Tensor.eqf) (@ln1 A zeroA coerZ addA subA mulA divA sqrtA default d_model eps ln1_w ln1_b r s)
+      := _.
+    #[export] Instance ln2_Proper {A zeroA coerZ addA subA mulA divA sqrtA default d_model eps ln2_w ln2_b r s}
+      : Proper (Tensor.eqf ==> Tensor.eqf) (@ln2 A zeroA coerZ addA subA mulA divA sqrtA default d_model eps ln2_w ln2_b r s)
+      := _.
+
+    #[export] Instance attn_only_out_Proper {A r batch zeroA coerZ addA subA mulA divA sqrtA expA default pos n_heads d_model d_head n_ctx use_split_qkv_input W_Q W_K W_V W_O b_Q b_K b_V b_O eps ln1_w ln1_b}
+      : Proper (Tensor.eqf ==> Tensor.eqf) (@attn_only_out A r batch zeroA coerZ addA subA mulA divA sqrtA expA default pos n_heads d_model d_head n_ctx use_split_qkv_input W_Q W_K W_V W_O b_Q b_K b_V b_O eps ln1_w ln1_b).
+    Proof.
+      cbv [attn_only_out]; t.
+      all: apply Attention.attn_out_Proper; t.
+      all: apply ln1_Proper; t.
+      all: first [ apply query_input_Proper | apply key_input_Proper | apply value_input_Proper ]; t.
+    Qed.
+  End TransformerBlock.
+  Export (hints) TransformerBlock.
+
+  Module HookedTransformer.
+    Export HookedTransformer.
+
+    #[export] Instance embed_Proper {A d_vocab d_model W_E r batch pos}
+      : Proper (Tensor.eqf ==> Tensor.eqf) (@embed A d_vocab d_model W_E r batch pos)
+      := _.
+    #[export] Instance pos_embed_Proper {A d_model n_ctx W_pos r batch pos}
+      : Proper (Tensor.eqf ==> Tensor.eqf) (@pos_embed A d_model n_ctx W_pos r batch pos)
+      := _.
+
+    #[export] Instance blocks_Proper {A zeroA coerZ addA subA mulA divA sqrtA expA default n_heads d_model d_head n_ctx eps blocks_params r batch pos}
+      : Proper (List.Forall2 (Tensor.eqf ==> Tensor.eqf))%signature (@blocks A zeroA coerZ addA subA mulA divA sqrtA expA default n_heads d_model d_head n_ctx eps blocks_params r batch pos).
+    Proof.
+      cbv [Proper blocks]; clear.
+      induction blocks_params as [|?? IH]; cbn [List.map]; constructor; auto; [].
+      destruct_head'_prod.
+      apply TransformerBlock.attn_only_out_Proper.
+    Qed.
+
+    #[export] Instance ln_final_Proper {A zeroA coerZ addA subA mulA divA sqrtA default d_model eps ln_final_w ln_final_b r batch pos}
+      : Proper (Tensor.eqf ==> Tensor.eqf) (@ln_final A zeroA coerZ addA subA mulA divA sqrtA default d_model eps ln_final_w ln_final_b r batch pos)
+      := _.
+
+    #[export] Instance unembed_Proper {A zeroA addA mulA d_vocab_out d_model W_U b_U r batch pos}
+      : Proper (Tensor.eqf ==> Tensor.eqf) (@unembed A zeroA addA mulA d_vocab_out d_model W_U b_U r batch pos)
+      := _.
+
+    #[export] Instance blocks_cps_Proper {A zeroA coerZ addA subA mulA divA sqrtA expA default n_heads d_model d_head n_ctx eps blocks_params r batch pos T R}
+      : Proper (Tensor.eqf ==> (Tensor.eqf ==> R) ==> R) (@blocks_cps A zeroA coerZ addA subA mulA divA sqrtA expA default n_heads d_model d_head n_ctx eps blocks_params r batch pos T).
+    Proof.
+      cbv [blocks_cps].
+      let blocks := lazymatch goal with |- context[fold_right _ _ ?ls] => ls end in
+      pose proof (blocks_Proper : List.Forall2 _ blocks blocks) as H;
+      induction blocks as [|?? IH]; inversion H; clear H; subst; cbn [fold_right]; [ now t | ].
+      repeat intro.
+      apply IH; clear IH; t; assumption.
+    Qed.
+
+    #[export] Instance logits_Proper {A zeroA coerZ addA subA mulA divA sqrtA expA default d_vocab d_vocab_out n_heads d_model d_head n_ctx eps W_E W_pos blocks_params ln_final_w ln_final_b W_U b_U r batch pos}
+      : Proper (Tensor.eqf ==> Tensor.eqf) (@logits A zeroA coerZ addA subA mulA divA sqrtA expA default d_vocab d_vocab_out n_heads d_model d_head n_ctx eps W_E W_pos blocks_params ln_final_w ln_final_b W_U b_U r batch pos).
+    Proof.
+      cbv [logits]; t.
+      refine (blocks_cps_Proper (R:=Tensor.eqf) _ _ _); t.
+      all: first [ apply embed_Proper | apply pos_embed_Proper | apply unembed_Proper ]; t.
+      apply ln_final_Proper; t.
+    Qed.
+
+    #[export] Instance forward_Proper {A zeroA coerZ addA subA mulA divA sqrtA expA default d_vocab d_vocab_out n_heads d_model d_head n_ctx eps W_E W_pos blocks_params ln_final_w ln_final_b W_U b_U r batch pos}
+      : Proper (Tensor.eqf ==> Tensor.eqf) (@forward A zeroA coerZ addA subA mulA divA sqrtA expA default d_vocab d_vocab_out n_heads d_model d_head n_ctx eps W_E W_pos blocks_params ln_final_w ln_final_b W_U b_U r batch pos)
+      := _.
+  End HookedTransformer.
+  Export (hints) HookedTransformer.
+End HookedTransformer.
+Export (hints) HookedTransformer.
