theories/Util/SolveProperEqRel.v
@@ -1,0 +1,23 @@
+From Coq Require Import Morphisms.
+
+Ltac make_eq_rel T :=
+  lazymatch T with
+  | (?A -> ?B)
+    => let RB := make_eq_rel B in
+      constr:(@respectful A B (@eq A) RB)
+  | (forall a : ?A, ?B)
+    => let B' := fresh in
+      constr:(@forall_relation A (fun a : A => B) (fun a : A => match B with B' => ltac:(let B'' := (eval cbv delta [B'] in B') in
+                                                                                  let RB := make_eq_rel B in
+                                                                                  exact RB) end))
+  | _ => constr:(@eq T)
+  end.
+Ltac solve_Proper_eq :=
+  match goal with
+  | [ |- @Proper ?A ?R ?f ]
+    => let R' := make_eq_rel A in
+      unify R R';
+      apply (@reflexive_proper A R')
+  end.
+
+#[export] Hint Extern 0 (Proper _ _) => solve_Proper_eq : typeclass_instances.
